theories/Type/Tactics.v
@@ -34,6 +34,7 @@ Ltac solve_subterm := intros;
 Ltac Equations.Init.solve_subterm ::= solve_subterm.
 Ltac Equations.Init.solve_eqdec ::= eqdec_proof.
 Ltac Equations.Init.unfold_recursor ::= Equations.Type.Subterm.unfold_recursor.
+Ltac Equations.Init.unfold_recursor_ext ::= Equations.Type.Subterm.unfold_recursor_ext.
 
 Ltac solve_noconf_prf := intros;
   on_last_hyp ltac:(fun id => destruct id) ; (* Subtitute a = b *)
